# Complex Rooting

$$
r = \sqrt[y]{x} = x ^ {\frac{1}{y}} ~~,~~
(x,y) \isin \R^2

\\~\\

x = |x| e ^{i(\theta + 2k\pi)}

\\~\\

r = \sqrt[y]{|x|}.e^{i\frac{\theta}{y}}.\sqrt[y]{e^{i2k\pi}}

\\~\\

r = \sqrt[y]{|x|} (\cos\frac{\theta}{y}+i\sin\frac{\theta}{y}) \sqrt[y]{1}

\\~\\

r =
\begin{cases}
	\sqrt[y]{x} \sqrt[y]{1} ~~,~~ x \ge 0
	\\~\\
	\sqrt[y]{-x} (\cos\frac{\pi}{y}+i\sin\frac{\pi}{y}) \sqrt[y]{1} ~~,~~ x < 0
\end{cases}

\\~\\

\boxed{
	r_0 =
	\begin{cases}
		\sqrt[y]{x} ~~,~~ x \ge 0
		\\~\\
		\sqrt[y]{-x} (\cos\frac{\pi}{y}+i\sin\frac{\pi}{y}) ~~,~~ x<0
	\end{cases}
}
$$

## Sample 1
$$
r = \sqrt[2]{-4} = \sqrt[2]{4} (\cos\frac{\pi}{2}+i\sin\frac{\pi}{2})

\\~\\

r = 2i \implies r^2 = -4

$$

## Sample 2
$$
r = \sqrt[-2]{-4} = \sqrt[-2]{4} (\cos\frac{\pi}{-2}+i\sin\frac{\pi}{-2})

\\~\\

r = \frac{-i}{2} \implies r^{-2} = (\frac{-1}{4})^{-1} = -4
$$
